intro step and deriving prover step from it

pulse/lib/steel/pulse/Pulse.Checker.Auto.Prover.fst
@@ -48,16 +48,188 @@ let init_prover_state (#g:env) (#ctxt:vprop) (ctxt_typing: vprop_typing g ctxt)
         proof_steps_typing=post_with_emp (proof_steps_idem_typing _ ctxt);
     }
 
-open FStar.List.Tot 
+open FStar.List.Tot
+
+let is_ghost_comp (c:comp) =
+  C_STGhost? c /\ comp_u c == u_zero /\ comp_res c == tm_unit
+
+//
+// result of an intro (pure, exists, rewrite) step
+//   that consumes some vprop v from p.unmatched_pre
+//
+noeq
+type intro_result (#g:env) (#ctxt:vprop) (p:prover_state g ctxt) = {
+  // the vprop that intro introduced
+  v : vprop;
+
+  // new unmatched pre and remaining ctxt
+  unmatched' : list vprop;
+  remaining' : list vprop;
+
+  // the term, comp, and term typing as a witness of the introduction
+  t' : st_term;
+  c' : c:comp { is_ghost_comp c /\ comp_post c == v };
+  t'_typing : st_typing g t' c';
+
+  // relation between new and old unmatched_pre and remaining_ctxt
+  unmatched_equiv : vprop_equiv g (list_as_vprop p.unmatched_pre)
+                                  (Tm_Star v (list_as_vprop unmatched'));
+  remaining_equiv : vprop_equiv g (list_as_vprop p.remaining_ctxt)
+                                  (Tm_Star (comp_pre c') (list_as_vprop remaining'));
+}
+
+
+let add_frame (#g:env) (#t:st_term) (#c:comp_st)
+  (d:st_typing g t c)
+  (f:vprop)
+  : c':comp { c' == Pulse.Typing.add_frame c f } &
+    st_typing g t c' = admit ()
+
+let with_pre_post (c:comp_st) (pre:vprop) (post:vprop) : comp_st =
+  match c with
+  | C_ST s
+  | C_STGhost _ s
+  | C_STAtomic _ s -> with_st_comp c { s with pre; post }
+
+let pre_equiv (#g:env) (#t:st_term) (#c:comp_st)
+  (d:st_typing g t c)
+  (f:vprop) (_:vprop_equiv g (comp_pre c) f)
+  : c':comp { c' == with_pre_post c f (comp_post c) } &
+    st_typing g t c' = admit ()
+
+//
+// note that we need post to be ln
+//
+let pre_post_equiv (#g:env) (#t:st_term) (#c:comp_st {ln (comp_post c)})
+  (d:st_typing g t c)
+  (#pre:vprop) (_:vprop_equiv g (comp_pre c) pre)
+  (#post:vprop) (_:vprop_equiv g (comp_post c) post)
+  : c':comp_st { c' == with_pre_post c pre post } &
+    st_typing g t c' = admit ()
+
+let st_typing_weakening (#g:env) (#t:st_term) (#c:comp)
+  (d:st_typing g t c)
+  (g':env { env_extends g' g })
+  : st_typing g' t c = admit ()
+
+
+//
+// derive next prover state from an intro step
+//
+#push-options "--z3rlimit_factor 30 --fuel 2 --ifuel 2"
+let get_next_prover_state (#g:env) (#ctxt:vprop) (#p:prover_state g ctxt)
+  (r:intro_result p)
+  : T.Tac (prover_state g ctxt) =
+  
+  let remaining'_matched = Tm_Star (list_as_vprop r.remaining') p.matched_pre in
+  let (| r_c', r_t'_typing |) = add_frame r.t'_typing remaining'_matched in
+  assert (comp_pre r_c' == Tm_Star (comp_pre r.c') remaining'_matched);
+  assert (comp_post r_c' == Tm_Star r.v remaining'_matched);
+
+  let (| x, bind_continuation_elaborator |) =
+    continuation_elaborator_with_bind #g Tm_Emp
+    #(ghost_comp ctxt (Tm_Star (list_as_vprop p.remaining_ctxt) p.matched_pre))
+    #p.proof_steps
+    p.proof_steps_typing
+    (magic () <: tot_typing g (Tm_Star Tm_Emp ctxt) Tm_VProp)
+  in
+
+  assume (open_term (Tm_Star (list_as_vprop p.remaining_ctxt) p.matched_pre) x ==
+                    Tm_Star (list_as_vprop p.remaining_ctxt) p.matched_pre);
+
+  let _ : vprop_equiv g (list_as_vprop p.remaining_ctxt)
+                        (Tm_Star (comp_pre r.c') (list_as_vprop r.remaining')) = r.remaining_equiv in
+  let d : vprop_equiv g
+    (Tm_Star (comp_pre r.c') (Tm_Star (list_as_vprop r.remaining') p.matched_pre))
+    (Tm_Star (Tm_Star (list_as_vprop p.remaining_ctxt) p.matched_pre) Tm_Emp) = magic () in
+
+  let (| r_c', r_t'_typing |) = pre_equiv r_t'_typing
+    (Tm_Star (Tm_Star (list_as_vprop p.remaining_ctxt) p.matched_pre) Tm_Emp)
+    d in
+
+  assume (env_extends (extend x (Inl tm_unit) g) g);
+  let r_t'_typing = st_typing_weakening r_t'_typing (extend x (Inl tm_unit) g) in
+
+  let post_hint = Some {
+    g;
+    ret_ty = tm_unit;
+    u = u_zero;
+    ty_typing = magic ();
+    post = comp_post r_c';
+    post_typing = magic ();
+  } in
+  assert (comp_post_matches_hint r_c' post_hint);
+  assume (env_extends g g);
+
+  let (| steps, steps_c, steps_typing |) = bind_continuation_elaborator post_hint
+    (| r.t', r_c', r_t'_typing  |) in
+
+  assume (stateful_comp steps_c);
+  assert (comp_pre steps_c == Tm_Star Tm_Emp ctxt);
+  assert (comp_post steps_c == comp_post r_c');
+  assume (steps_c == ghost_comp (Tm_Star Tm_Emp ctxt) (comp_post r_c'));
+  assume (ln (comp_post steps_c));
+
+  let new_matched = Tm_Star p.matched_pre r.v in
+  let new_unmatched = r.unmatched' in
+  let new_remaining = r.remaining' in
+
+  assert (comp_post steps_c ==
+          Tm_Star r.v (Tm_Star (list_as_vprop r.remaining') p.matched_pre));
+  
+  let steps_pre_equiv : vprop_equiv g (Tm_Star Tm_Emp ctxt) ctxt = magic () in
+  let steps_post_equiv : vprop_equiv g
+    (Tm_Star r.v (Tm_Star (list_as_vprop r.remaining') p.matched_pre))
+    (Tm_Star (list_as_vprop r.remaining') (Tm_Star p.matched_pre r.v)) = magic () in
+
+  let (| steps_c, steps_typing |) = pre_post_equiv steps_typing
+    steps_pre_equiv
+    steps_post_equiv in
+
+  assert (comp_pre steps_c == ctxt);
+  assert (comp_post steps_c == Tm_Star (list_as_vprop r.remaining')
+                                       (Tm_Star p.matched_pre r.v));
+  assume (steps_c == ghost_comp ctxt (Tm_Star (list_as_vprop r.remaining')
+                                              (Tm_Star p.matched_pre r.v)));
+
+  let d1 : vprop_equiv g (comp_pre p.c)
+                         (Tm_Star (list_as_vprop p.unmatched_pre) p.matched_pre) = p.pre_equiv in
+  let d2 : vprop_equiv g (list_as_vprop p.unmatched_pre)
+                         (Tm_Star r.v (list_as_vprop r.unmatched')) = r.unmatched_equiv in
+  let d3 : vprop_equiv g (comp_pre p.c) (Tm_Star (list_as_vprop r.unmatched')
+                                                 (Tm_Star p.matched_pre r.v)) = magic () in
+
+  { p with
+    matched_pre = Tm_Star p.matched_pre r.v;
+    unmatched_pre = r.unmatched';
+    remaining_ctxt = r.remaining';
+    proof_steps = steps;
+    proof_steps_typing = steps_typing;
+    pre_equiv = d3 }
+#pop-options
 
 let tm_prop = Tm_FStar FStar.Reflection.Typing.tm_prop Range.range_0
-let step_intro_one_pure #g (goal:term) (d:tot_typing g goal tm_prop)
-  : prover_step_t 
-  = fun #g #o p -> None
 
-let step_intro_exists #g #o (p:prover_state g o) : T.Tac (option (prover_state g o)) = None
-let step_intro_pure #g #o (p:prover_state g o) : T.Tac (option (prover_state g o)) = None
-let step_intro_rewrite #g #o (p:prover_state g o) : T.Tac (option (prover_state g o)) = None
+type intro_step_t =
+  #g:env -> #ctxt:vprop ->
+  p:prover_state g ctxt ->
+  T.Tac (option (intro_result p))
+
+assume val step_intro_exists : intro_step_t
+assume val step_intro_pure : intro_step_t
+assume val step_intro_rewrite : intro_step_t
+
+let prover_step_intro_exists #g #o (p:prover_state g o)
+  : T.Tac (option (prover_state g o)) =
+  T.map_opt get_next_prover_state (step_intro_exists p)
+
+let prover_step_intro_pure #g #o (p:prover_state g o)
+  : T.Tac (option (prover_state g o)) =
+  T.map_opt get_next_prover_state (step_intro_pure p)
+
+let prover_step_intro_rewrite #g #o (p:prover_state g o)
+  : T.Tac (option (prover_state g o)) =
+  T.map_opt get_next_prover_state (step_intro_rewrite p)
 
 let rec first_success (l:list prover_step_t) : prover_step_t = 
   fun #g #o p ->
@@ -72,9 +244,9 @@ let rec first_success (l:list prover_step_t) : prover_step_t =
    If neither, then returns None; and the outer loop should fail reporting unmatched preconditions *)
 let step : prover_step_t
   = first_success [ Pulse.Checker.Auto.Framing.step_match <: prover_step_t;
-                    step_intro_exists <: prover_step_t;
-                    step_intro_pure <: prover_step_t;
-                    step_intro_rewrite <: prover_step_t ]
+                    prover_step_intro_exists <: prover_step_t;
+                    prover_step_intro_pure <: prover_step_t;
+                    prover_step_intro_rewrite <: prover_step_t ]
 
 let finish #g #o (p:prover_state g o { p.unmatched_pre == []})
   : (t:st_term & c:comp_st { comp_pre c == o } & st_typing g t c)
